Autosubst4Lean/Test4/Substitution.lean
@@ -1,10 +1,11 @@
-import Autosubst4Lean.Test2.Syntax
+import Autosubst4Lean.Test4.Syntax
 
-namespace Fsub
+namespace RegionCalc
 
 structure Subst (s1 s2 : Sig) where
   var : BVar s1 .var -> Exp s2
   tvar : BVar s1 .tvar -> Ty s2
+  rvar : BVar s1 .rvar -> BVar s2 .rvar
 
 def Subst.lift (σ : Subst s1 s2) : Subst (s1,,k) (s2,,k) where
   var := fun x => by
@@ -15,6 +16,10 @@ def Subst.lift (σ : Subst s1 s2) : Subst (s1,,k) (s2,,k) where
     cases x
     case here => exact .tvar .here
     case there x => exact (σ.tvar x).rename Rename.succ
+  rvar := fun x => by
+    cases x
+    case here => exact .here
+    case there x => exact (σ.rvar x).there
 
 def Subst.liftMany (σ : Subst s1 s2) (K : Sig) : Subst (s1 ++ K) (s2 ++ K) :=
   match K with
@@ -24,33 +29,47 @@ def Subst.liftMany (σ : Subst s1 s2) (K : Sig) : Subst (s1 ++ K) (s2 ++ K) :=
 def Subst.id {s : Sig} : Subst s s where
   var := fun x => .var x
   tvar := fun x => .tvar x
+  rvar := fun x => x
 
 def Ty.subst : Ty s1 -> Subst s1 s2 -> Ty s2
-| .top, _ => .top
 | .tvar x0, σ => σ.tvar x0
 | .arrow a0 a1, σ => .arrow (a0.subst σ) (a1.subst σ)
-| .forall_ a0 a1, σ => .forall_ (a0.subst σ) (a1.subst σ.lift)
+| .ref x0 a1, σ => .ref (σ.rvar x0) (a1.subst σ)
+| .forallTy a0, σ => .forallTy (a0.subst σ.lift)
+| .forallRgn a0, σ => .forallRgn (a0.subst σ.lift)
+| .unit, _ => .unit
 
 def Exp.subst : Exp s1 -> Subst s1 s2 -> Exp s2
 | .var x0, σ => σ.var x0
 | .abs a0 a1, σ => .abs (a0.subst σ) (a1.subst σ.lift)
 | .app a0 a1, σ => .app (a0.subst σ) (a1.subst σ)
-| .tabs a0 a1, σ => .tabs (a0.subst σ) (a1.subst σ.lift)
+| .tabs a0, σ => .tabs (a0.subst σ.lift)
 | .tapp a0 a1, σ => .tapp (a0.subst σ) (a1.subst σ)
+| .rabs a0, σ => .rabs (a0.subst σ.lift)
+| .rapp a0 x1, σ => .rapp (a0.subst σ) (σ.rvar x1)
+| .new x0 a1, σ => .new (σ.rvar x0) (a1.subst σ)
+| .deref a0, σ => .deref (a0.subst σ)
+| .assign a0 a1, σ => .assign (a0.subst σ) (a1.subst σ)
+| .letrgn a0, σ => .letrgn (a0.subst σ.lift)
+| .unit, _ => .unit
 
 theorem Subst.funext {σ1 σ2 : Subst s1 s2}
   (hvar : ∀ x, σ1.var x = σ2.var x)
   (htvar : ∀ x, σ1.tvar x = σ2.tvar x)
+  (hrvar : ∀ x, σ1.rvar x = σ2.rvar x)
   : σ1 = σ2 := by
   cases σ1; cases σ2
   simp only [Subst.mk.injEq]
   constructor
   · funext x; exact hvar x
+  constructor
   · funext x; exact htvar x
+  · funext x; exact hrvar x
 
 def Subst.comp (σ1 : Subst s1 s2) (σ2 : Subst s2 s3) : Subst s1 s3 where
   var := fun x => (σ1.var x).subst σ2
   tvar := fun x => (σ1.tvar x).subst σ2
+  rvar := fun x => σ2.rvar (σ1.rvar x)
 
 theorem Subst.lift_there_var_eq {σ : Subst s1 s2} {x : BVar s1 .var} :
   (σ.lift (k:=k)).var (.there x) = (σ.var x).rename Rename.succ := by
@@ -60,11 +79,19 @@ theorem Subst.lift_there_tvar_eq {σ : Subst s1 s2} {x : BVar s1 .tvar} :
   (σ.lift (k:=k)).tvar (.there x) = (σ.tvar x).rename Rename.succ := by
   rfl
 
+theorem Subst.lift_there_rvar_eq {σ : Subst s1 s2} {x : BVar s1 .rvar} :
+  (σ.lift (k:=k)).rvar (.there x) = (σ.rvar x).there := by
+  rfl
+
 theorem Rename.lift_there_var_eq {f : Rename s1 s2} {x : BVar s1 .var} :
   (f.lift (k:=k)).var (.there x) = (f.var x).there := by
   rfl
 
 theorem Rename.lift_there_tvar_eq {f : Rename s1 s2} {x : BVar s1 .tvar} :
+  (f.lift (k:=k)).var (.there x) = (f.var x).there := by
+  rfl
+
+theorem Rename.lift_there_rvar_eq {f : Rename s1 s2} {x : BVar s1 .rvar} :
   (f.lift (k:=k)).var (.there x) = (f.var x).there := by
   rfl
 
@@ -114,11 +141,27 @@ theorem Tvar.weaken_subst_comm_liftMany {x : BVar (s1 ++ K) .tvar} {σ : Subst s
       simp [Ty.weaken_rename_comm]
       grind
 
+theorem Rvar.weaken_subst_comm_liftMany {x : BVar (s1 ++ K) .rvar} {σ : Subst s1 s2} :
+  (((Rename.succ (k:=k0)).liftMany K).var ((σ.liftMany K).rvar x)) =
+  (σ.lift (k:=k0).liftMany K).rvar (((Rename.succ (k:=k0)).liftMany K).var x) := by
+  induction K with
+  | nil =>
+    simp [Subst.liftMany, Rename.liftMany]
+    cases x with
+    | here => simp [Subst.lift, Rename.succ]
+    | there x => rfl
+  | cons k K ih =>
+    simp [Subst.liftMany, Rename.liftMany]
+    cases x with
+    | here => rfl
+    | there x =>
+      simp only [Rename.lift_there_rvar_eq, Subst.lift_there_rvar_eq]
+      exact congrArg BVar.there ih
+
 theorem Ty.weaken_subst_comm {t : Ty (s1 ++ K)} {σ : Subst s1 s2} :
   (t.subst (σ.liftMany K)).rename ((Rename.succ (k:=k0)).liftMany K) =
   (t.rename ((Rename.succ (k:=k0)).liftMany K)).subst (σ.lift (k:=k0).liftMany K) := by
   match t with
-  | .top => rfl
   | .tvar x =>
     simp [Ty.subst, Ty.rename]
     exact Tvar.weaken_subst_comm_liftMany
@@ -126,11 +169,18 @@ theorem Ty.weaken_subst_comm {t : Ty (s1 ++ K)} {σ : Subst s1 s2} :
     have ih0 := Ty.weaken_subst_comm (t:=f0) (σ:=σ) (K:=K) (k0:=k0)
     have ih1 := Ty.weaken_subst_comm (t:=f1) (σ:=σ) (K:=K) (k0:=k0)
     simp [Ty.subst, Ty.rename, ih0, ih1]
-  | .forall_ f0 f1 =>
-    have ih0 := Ty.weaken_subst_comm (t:=f0) (σ:=σ) (K:=K) (k0:=k0)
-    have ih1 := Ty.weaken_subst_comm (t:=f1) (σ:=σ) (K:=K,X) (k0:=k0)
-    simp [Ty.subst, Ty.rename, ih0]
-    exact ih1
+  | .ref _ f1 =>
+    have ih1 := Ty.weaken_subst_comm (t:=f1) (σ:=σ) (K:=K) (k0:=k0)
+    simp [Ty.subst, Ty.rename, ih1, Rvar.weaken_subst_comm_liftMany]
+  | .forallTy f0 =>
+    have ih0 := Ty.weaken_subst_comm (t:=f0) (σ:=σ) (K:=K,X) (k0:=k0)
+    simp [Ty.subst, Ty.rename]
+    exact ih0
+  | .forallRgn f0 =>
+    have ih0 := Ty.weaken_subst_comm (t:=f0) (σ:=σ) (K:=K,r) (k0:=k0)
+    simp [Ty.subst, Ty.rename]
+    exact ih0
+  | .unit => rfl
 
 theorem Ty.weaken_subst_comm_base {t : Ty s1} {σ : Subst s1 s2} :
   (t.subst σ).rename (Rename.succ (k:=k0)) = (t.rename Rename.succ).subst (σ.lift (k:=k0)) :=
@@ -152,15 +202,36 @@ theorem Exp.weaken_subst_comm {t : Exp (s1 ++ K)} {σ : Subst s1 s2} :
     have ih0 := Exp.weaken_subst_comm (t:=f0) (σ:=σ) (K:=K) (k0:=k0)
     have ih1 := Exp.weaken_subst_comm (t:=f1) (σ:=σ) (K:=K) (k0:=k0)
     simp [Exp.subst, Exp.rename, ih0, ih1]
-  | .tabs f0 f1 =>
-    have ih0 := Ty.weaken_subst_comm (t:=f0) (σ:=σ) (K:=K) (k0:=k0)
-    have ih1 := Exp.weaken_subst_comm (t:=f1) (σ:=σ) (K:=K,X) (k0:=k0)
-    simp [Exp.subst, Exp.rename, ih0]
-    exact ih1
+  | .tabs f0 =>
+    have ih0 := Exp.weaken_subst_comm (t:=f0) (σ:=σ) (K:=K,X) (k0:=k0)
+    simp [Exp.subst, Exp.rename]
+    exact ih0
   | .tapp f0 f1 =>
     have ih0 := Exp.weaken_subst_comm (t:=f0) (σ:=σ) (K:=K) (k0:=k0)
     have ih1 := Ty.weaken_subst_comm (t:=f1) (σ:=σ) (K:=K) (k0:=k0)
     simp [Exp.subst, Exp.rename, ih0, ih1]
+  | .rabs f0 =>
+    have ih0 := Exp.weaken_subst_comm (t:=f0) (σ:=σ) (K:=K,r) (k0:=k0)
+    simp [Exp.subst, Exp.rename]
+    exact ih0
+  | .rapp f0 _ =>
+    have ih0 := Exp.weaken_subst_comm (t:=f0) (σ:=σ) (K:=K) (k0:=k0)
+    simp [Exp.subst, Exp.rename, ih0, Rvar.weaken_subst_comm_liftMany]
+  | .new _ f1 =>
+    have ih1 := Exp.weaken_subst_comm (t:=f1) (σ:=σ) (K:=K) (k0:=k0)
+    simp [Exp.subst, Exp.rename, ih1, Rvar.weaken_subst_comm_liftMany]
+  | .deref f0 =>
+    have ih0 := Exp.weaken_subst_comm (t:=f0) (σ:=σ) (K:=K) (k0:=k0)
+    simp [Exp.subst, Exp.rename, ih0]
+  | .assign f0 f1 =>
+    have ih0 := Exp.weaken_subst_comm (t:=f0) (σ:=σ) (K:=K) (k0:=k0)
+    have ih1 := Exp.weaken_subst_comm (t:=f1) (σ:=σ) (K:=K) (k0:=k0)
+    simp [Exp.subst, Exp.rename, ih0, ih1]
+  | .letrgn f0 =>
+    have ih0 := Exp.weaken_subst_comm (t:=f0) (σ:=σ) (K:=K,r) (k0:=k0)
+    simp [Exp.subst, Exp.rename]
+    exact ih0
+  | .unit => rfl
 
 theorem Exp.weaken_subst_comm_base {t : Exp s1} {σ : Subst s1 s2} :
   (t.subst σ).rename (Rename.succ (k:=k0)) = (t.rename Rename.succ).subst (σ.lift (k:=k0)) :=
@@ -185,6 +256,8 @@ theorem Subst.comp_lift {σ1 : Subst s1 s2} {σ2 : Subst s2 s3} {k : Kind} :
         lhs; simp only [Subst.comp, Subst.lift_there_tvar_eq]
       simp only [Subst.lift_there_tvar_eq]
       simp only [Ty.weaken_subst_comm_base, Subst.comp]
+  · intro x
+    cases x <;> rfl
 
 theorem Subst.comp_liftMany {σ1 : Subst s1 s2} {σ2 : Subst s2 s3} {K : Sig} :
   (σ1.liftMany K).comp (σ2.liftMany K) = (σ1.comp σ2).liftMany K := by
@@ -197,12 +270,16 @@ theorem Subst.comp_liftMany {σ1 : Subst s1 s2} {σ2 : Subst s2 s3} {K : Sig} :
 theorem Ty.subst_comp {t : Ty s1} {σ1 : Subst s1 s2} {σ2 : Subst s2 s3} :
   (t.subst σ1).subst σ2 = t.subst (σ1.comp σ2) := by
   induction t generalizing s2 s3 with
-  | top => rfl
   | tvar => simp [Ty.subst, Subst.comp]
   | arrow _ _ ih0 ih1 =>
     simp_all [Ty.subst]
-  | forall_ _ _ ih0 ih1 =>
+  | ref _ _ ih0 =>
+    simp_all [Ty.subst, Subst.comp]
+  | forallTy _ ih0 =>
     simp_all [Ty.subst, Subst.comp_lift]
+  | forallRgn _ ih0 =>
+    simp_all [Ty.subst, Subst.comp_lift]
+  | unit => rfl
 
 theorem Exp.subst_comp {t : Exp s1} {σ1 : Subst s1 s2} {σ2 : Subst s2 s3} :
   (t.subst σ1).subst σ2 = t.subst (σ1.comp σ2) := by
@@ -212,10 +289,23 @@ theorem Exp.subst_comp {t : Exp s1} {σ1 : Subst s1 s2} {σ2 : Subst s2 s3} :
     simp_all [Exp.subst, Ty.subst_comp, Subst.comp_lift]
   | app _ _ ih0 ih1 =>
     simp_all [Exp.subst]
-  | tabs _ _ ih0 =>
-    simp_all [Exp.subst, Ty.subst_comp, Subst.comp_lift]
+  | tabs _ ih0 =>
+    simp_all [Exp.subst, Subst.comp_lift]
   | tapp _ _ ih0 =>
     simp_all [Exp.subst, Ty.subst_comp]
+  | rabs _ ih0 =>
+    simp_all [Exp.subst, Subst.comp_lift]
+  | rapp _ _ ih0 =>
+    simp_all [Exp.subst, Subst.comp]
+  | new _ _ ih0 =>
+    simp_all [Exp.subst, Subst.comp]
+  | deref _ ih0 =>
+    simp_all [Exp.subst]
+  | assign _ _ ih0 ih1 =>
+    simp_all [Exp.subst]
+  | letrgn _ ih0 =>
+    simp_all [Exp.subst, Subst.comp_lift]
+  | unit => rfl
 
 theorem Subst.lift_id :
   (Subst.id (s:=s)).lift (k:=k) = Subst.id := by
@@ -224,16 +314,22 @@ theorem Subst.lift_id :
     cases x <;> rfl
   · intro x
     cases x <;> rfl
+  · intro x
+    cases x <;> rfl
 
 theorem Ty.subst_id {t : Ty s} :
   t.subst Subst.id = t := by
   induction t with
-  | top => rfl
   | tvar => simp [Ty.subst, Subst.id]
   | arrow _ _ ih0 ih1 =>
     simp_all [Ty.subst]
-  | forall_ _ _ ih0 ih1 =>
+  | ref _ _ ih0 =>
+    simp_all [Ty.subst, Subst.id]
+  | forallTy _ ih0 =>
     simp_all [Ty.subst, Subst.lift_id]
+  | forallRgn _ ih0 =>
+    simp_all [Ty.subst, Subst.lift_id]
+  | unit => rfl
 
 theorem Exp.subst_id {t : Exp s} :
   t.subst Subst.id = t := by
@@ -243,9 +339,22 @@ theorem Exp.subst_id {t : Exp s} :
     simp_all [Exp.subst, Ty.subst_id, Subst.lift_id]
   | app _ _ ih0 ih1 =>
     simp_all [Exp.subst]
-  | tabs _ _ ih0 =>
-    simp_all [Exp.subst, Ty.subst_id, Subst.lift_id]
+  | tabs _ ih0 =>
+    simp_all [Exp.subst, Subst.lift_id]
   | tapp _ _ ih0 =>
     simp_all [Exp.subst, Ty.subst_id]
+  | rabs _ ih0 =>
+    simp_all [Exp.subst, Subst.lift_id]
+  | rapp _ _ ih0 =>
+    simp_all [Exp.subst, Subst.id]
+  | new _ _ ih0 =>
+    simp_all [Exp.subst, Subst.id]
+  | deref _ ih0 =>
+    simp_all [Exp.subst]
+  | assign _ _ ih0 ih1 =>
+    simp_all [Exp.subst]
+  | letrgn _ ih0 =>
+    simp_all [Exp.subst, Subst.lift_id]
+  | unit => rfl
 
-end Fsub
+end RegionCalc
