Autosubst4Lean/Test6/Substitution.lean
@@ -1,20 +1,15 @@
-import Autosubst4Lean.Test2.Syntax
+import Autosubst4Lean.Test6.Syntax
 
-namespace Fsub
+namespace MiniML
 
 structure Subst (s1 s2 : Sig) where
   var : BVar s1 .var -> Exp s2
-  tvar : BVar s1 .tvar -> Ty s2
 
 def Subst.lift (σ : Subst s1 s2) : Subst (s1,,k) (s2,,k) where
   var := fun x => by
     cases x
     case here => exact .var .here
     case there x => exact (σ.var x).rename Rename.succ
-  tvar := fun x => by
-    cases x
-    case here => exact .tvar .here
-    case there x => exact (σ.tvar x).rename Rename.succ
 
 def Subst.liftMany (σ : Subst s1 s2) (K : Sig) : Subst (s1 ++ K) (s2 ++ K) :=
   match K with
@@ -23,58 +18,57 @@ def Subst.liftMany (σ : Subst s1 s2) (K : Sig) : Subst (s1 ++ K) (s2 ++ K) :=
 
 def Subst.id {s : Sig} : Subst s s where
   var := fun x => .var x
-  tvar := fun x => .tvar x
 
 def Ty.subst : Ty s1 -> Subst s1 s2 -> Ty s2
-| .top, _ => .top
-| .tvar x0, σ => σ.tvar x0
+| .base, _ => .base
 | .arrow a0 a1, σ => .arrow (a0.subst σ) (a1.subst σ)
-| .forall_ a0 a1, σ => .forall_ (a0.subst σ) (a1.subst σ.lift)
+| .prod a0 a1, σ => .prod (a0.subst σ) (a1.subst σ)
+| .sum a0 a1, σ => .sum (a0.subst σ) (a1.subst σ)
+| .list a0, σ => .list (a0.subst σ)
+| .unit, _ => .unit
 
 def Exp.subst : Exp s1 -> Subst s1 s2 -> Exp s2
 | .var x0, σ => σ.var x0
 | .abs a0 a1, σ => .abs (a0.subst σ) (a1.subst σ.lift)
 | .app a0 a1, σ => .app (a0.subst σ) (a1.subst σ)
-| .tabs a0 a1, σ => .tabs (a0.subst σ) (a1.subst σ.lift)
-| .tapp a0 a1, σ => .tapp (a0.subst σ) (a1.subst σ)
+| .let_ a0 a1, σ => .let_ (a0.subst σ) (a1.subst σ.lift)
+| .letrec a0 a1 a2, σ => .letrec (a0.subst σ) (a1.subst σ.lift) (a2.subst σ.lift)
+| .pair a0 a1, σ => .pair (a0.subst σ) (a1.subst σ)
+| .fst a0, σ => .fst (a0.subst σ)
+| .snd a0, σ => .snd (a0.subst σ)
+| .inl a0, σ => .inl (a0.subst σ)
+| .inr a0, σ => .inr (a0.subst σ)
+| .case_ a0 a1 a2, σ => .case_ (a0.subst σ) (a1.subst σ.lift) (a2.subst σ.lift)
+| .nil, _ => .nil
+| .cons a0 a1, σ => .cons (a0.subst σ) (a1.subst σ)
+| .foldr a0 a1 a2, σ => .foldr (a0.subst σ) (a1.subst σ) (a2.subst σ)
+| .unit, _ => .unit
+| .fix a0, σ => .fix (a0.subst σ.lift)
+| .num a0, _ => .num a0
+| .succ a0, σ => .succ (a0.subst σ)
+| .ifz a0 a1 a2, σ => .ifz (a0.subst σ) (a1.subst σ) (a2.subst σ.lift)
 
 theorem Subst.funext {σ1 σ2 : Subst s1 s2}
   (hvar : ∀ x, σ1.var x = σ2.var x)
-  (htvar : ∀ x, σ1.tvar x = σ2.tvar x)
   : σ1 = σ2 := by
   cases σ1; cases σ2
   simp only [Subst.mk.injEq]
-  constructor
-  · funext x; exact hvar x
-  · funext x; exact htvar x
+  funext x; exact hvar x
 
 def Subst.comp (σ1 : Subst s1 s2) (σ2 : Subst s2 s3) : Subst s1 s3 where
   var := fun x => (σ1.var x).subst σ2
-  tvar := fun x => (σ1.tvar x).subst σ2
 
 theorem Subst.lift_there_var_eq {σ : Subst s1 s2} {x : BVar s1 .var} :
   (σ.lift (k:=k)).var (.there x) = (σ.var x).rename Rename.succ := by
-  rfl
-
-theorem Subst.lift_there_tvar_eq {σ : Subst s1 s2} {x : BVar s1 .tvar} :
-  (σ.lift (k:=k)).tvar (.there x) = (σ.tvar x).rename Rename.succ := by
   rfl
 
 theorem Rename.lift_there_var_eq {f : Rename s1 s2} {x : BVar s1 .var} :
   (f.lift (k:=k)).var (.there x) = (f.var x).there := by
   rfl
 
-theorem Rename.lift_there_tvar_eq {f : Rename s1 s2} {x : BVar s1 .tvar} :
-  (f.lift (k:=k)).var (.there x) = (f.var x).there := by
-  rfl
-
 theorem Exp.weaken_rename_comm {t : Exp s1} {f : Rename s1 s2} :
   (t.rename Rename.succ).rename (f.lift (k:=k0)) = (t.rename f).rename (Rename.succ) := by
   simp [Exp.rename_comp, Rename.succ_lift_comm]
-
-theorem Ty.weaken_rename_comm {t : Ty s1} {f : Rename s1 s2} :
-  (t.rename Rename.succ).rename (f.lift (k:=k0)) = (t.rename f).rename (Rename.succ) := by
-  simp [Ty.rename_comp, Rename.succ_lift_comm]
 
 theorem Var.weaken_subst_comm_liftMany {x : BVar (s1 ++ K) .var} {σ : Subst s1 s2} :
   ((σ.liftMany K).var x).rename ((Rename.succ (k:=k0)).liftMany K) =
@@ -95,42 +89,27 @@ theorem Var.weaken_subst_comm_liftMany {x : BVar (s1 ++ K) .var} {σ : Subst s1 
       simp [Exp.weaken_rename_comm]
       grind
 
-theorem Tvar.weaken_subst_comm_liftMany {x : BVar (s1 ++ K) .tvar} {σ : Subst s1 s2} :
-  ((σ.liftMany K).tvar x).rename ((Rename.succ (k:=k0)).liftMany K) =
-  (σ.lift (k:=k0).liftMany K).tvar (((Rename.succ (k:=k0)).liftMany K).var x) := by
-  induction K with
-  | nil =>
-    simp [Subst.liftMany, Rename.liftMany]
-    cases x with
-    | here => simp [Subst.lift, Rename.succ]
-    | there x => rfl
-  | cons k K ih =>
-    simp [Subst.liftMany, Rename.liftMany]
-    cases x with
-    | here => rfl
-    | there x =>
-      simp [Rename.lift_there_tvar_eq]
-      simp [Subst.lift_there_tvar_eq]
-      simp [Ty.weaken_rename_comm]
-      grind
-
 theorem Ty.weaken_subst_comm {t : Ty (s1 ++ K)} {σ : Subst s1 s2} :
   (t.subst (σ.liftMany K)).rename ((Rename.succ (k:=k0)).liftMany K) =
   (t.rename ((Rename.succ (k:=k0)).liftMany K)).subst (σ.lift (k:=k0).liftMany K) := by
   match t with
-  | .top => rfl
-  | .tvar x =>
-    simp [Ty.subst, Ty.rename]
-    exact Tvar.weaken_subst_comm_liftMany
+  | .base => rfl
   | .arrow f0 f1 =>
     have ih0 := Ty.weaken_subst_comm (t:=f0) (σ:=σ) (K:=K) (k0:=k0)
     have ih1 := Ty.weaken_subst_comm (t:=f1) (σ:=σ) (K:=K) (k0:=k0)
     simp [Ty.subst, Ty.rename, ih0, ih1]
-  | .forall_ f0 f1 =>
+  | .prod f0 f1 =>
     have ih0 := Ty.weaken_subst_comm (t:=f0) (σ:=σ) (K:=K) (k0:=k0)
-    have ih1 := Ty.weaken_subst_comm (t:=f1) (σ:=σ) (K:=K,X) (k0:=k0)
+    have ih1 := Ty.weaken_subst_comm (t:=f1) (σ:=σ) (K:=K) (k0:=k0)
+    simp [Ty.subst, Ty.rename, ih0, ih1]
+  | .sum f0 f1 =>
+    have ih0 := Ty.weaken_subst_comm (t:=f0) (σ:=σ) (K:=K) (k0:=k0)
+    have ih1 := Ty.weaken_subst_comm (t:=f1) (σ:=σ) (K:=K) (k0:=k0)
+    simp [Ty.subst, Ty.rename, ih0, ih1]
+  | .list f0 =>
+    have ih0 := Ty.weaken_subst_comm (t:=f0) (σ:=σ) (K:=K) (k0:=k0)
     simp [Ty.subst, Ty.rename, ih0]
-    exact ih1
+  | .unit => rfl
 
 theorem Ty.weaken_subst_comm_base {t : Ty s1} {σ : Subst s1 s2} :
   (t.subst σ).rename (Rename.succ (k:=k0)) = (t.rename Rename.succ).subst (σ.lift (k:=k0)) :=
@@ -152,15 +131,64 @@ theorem Exp.weaken_subst_comm {t : Exp (s1 ++ K)} {σ : Subst s1 s2} :
     have ih0 := Exp.weaken_subst_comm (t:=f0) (σ:=σ) (K:=K) (k0:=k0)
     have ih1 := Exp.weaken_subst_comm (t:=f1) (σ:=σ) (K:=K) (k0:=k0)
     simp [Exp.subst, Exp.rename, ih0, ih1]
-  | .tabs f0 f1 =>
-    have ih0 := Ty.weaken_subst_comm (t:=f0) (σ:=σ) (K:=K) (k0:=k0)
-    have ih1 := Exp.weaken_subst_comm (t:=f1) (σ:=σ) (K:=K,X) (k0:=k0)
+  | .let_ f0 f1 =>
+    have ih0 := Exp.weaken_subst_comm (t:=f0) (σ:=σ) (K:=K) (k0:=k0)
+    have ih1 := Exp.weaken_subst_comm (t:=f1) (σ:=σ) (K:=K,x) (k0:=k0)
     simp [Exp.subst, Exp.rename, ih0]
     exact ih1
-  | .tapp f0 f1 =>
+  | .letrec f0 f1 f2 =>
+    have ih0 := Ty.weaken_subst_comm (t:=f0) (σ:=σ) (K:=K) (k0:=k0)
+    have ih1 := Exp.weaken_subst_comm (t:=f1) (σ:=σ) (K:=K,x) (k0:=k0)
+    have ih2 := Exp.weaken_subst_comm (t:=f2) (σ:=σ) (K:=K,x) (k0:=k0)
+    simp [Exp.subst, Exp.rename, ih0]
+    exact ⟨ih1, ih2⟩
+  | .pair f0 f1 =>
     have ih0 := Exp.weaken_subst_comm (t:=f0) (σ:=σ) (K:=K) (k0:=k0)
-    have ih1 := Ty.weaken_subst_comm (t:=f1) (σ:=σ) (K:=K) (k0:=k0)
+    have ih1 := Exp.weaken_subst_comm (t:=f1) (σ:=σ) (K:=K) (k0:=k0)
     simp [Exp.subst, Exp.rename, ih0, ih1]
+  | .fst f0 =>
+    have ih0 := Exp.weaken_subst_comm (t:=f0) (σ:=σ) (K:=K) (k0:=k0)
+    simp [Exp.subst, Exp.rename, ih0]
+  | .snd f0 =>
+    have ih0 := Exp.weaken_subst_comm (t:=f0) (σ:=σ) (K:=K) (k0:=k0)
+    simp [Exp.subst, Exp.rename, ih0]
+  | .inl f0 =>
+    have ih0 := Exp.weaken_subst_comm (t:=f0) (σ:=σ) (K:=K) (k0:=k0)
+    simp [Exp.subst, Exp.rename, ih0]
+  | .inr f0 =>
+    have ih0 := Exp.weaken_subst_comm (t:=f0) (σ:=σ) (K:=K) (k0:=k0)
+    simp [Exp.subst, Exp.rename, ih0]
+  | .case_ f0 f1 f2 =>
+    have ih0 := Exp.weaken_subst_comm (t:=f0) (σ:=σ) (K:=K) (k0:=k0)
+    have ih1 := Exp.weaken_subst_comm (t:=f1) (σ:=σ) (K:=K,x) (k0:=k0)
+    have ih2 := Exp.weaken_subst_comm (t:=f2) (σ:=σ) (K:=K,x) (k0:=k0)
+    simp [Exp.subst, Exp.rename, ih0]
+    exact ⟨ih1, ih2⟩
+  | .nil => rfl
+  | .cons f0 f1 =>
+    have ih0 := Exp.weaken_subst_comm (t:=f0) (σ:=σ) (K:=K) (k0:=k0)
+    have ih1 := Exp.weaken_subst_comm (t:=f1) (σ:=σ) (K:=K) (k0:=k0)
+    simp [Exp.subst, Exp.rename, ih0, ih1]
+  | .foldr f0 f1 f2 =>
+    have ih0 := Exp.weaken_subst_comm (t:=f0) (σ:=σ) (K:=K) (k0:=k0)
+    have ih1 := Exp.weaken_subst_comm (t:=f1) (σ:=σ) (K:=K) (k0:=k0)
+    have ih2 := Exp.weaken_subst_comm (t:=f2) (σ:=σ) (K:=K) (k0:=k0)
+    simp [Exp.subst, Exp.rename, ih0, ih1, ih2]
+  | .unit => rfl
+  | .fix f0 =>
+    have ih0 := Exp.weaken_subst_comm (t:=f0) (σ:=σ) (K:=K,x) (k0:=k0)
+    simp [Exp.subst, Exp.rename]
+    exact ih0
+  | .num _ => rfl
+  | .succ f0 =>
+    have ih0 := Exp.weaken_subst_comm (t:=f0) (σ:=σ) (K:=K) (k0:=k0)
+    simp [Exp.subst, Exp.rename, ih0]
+  | .ifz f0 f1 f2 =>
+    have ih0 := Exp.weaken_subst_comm (t:=f0) (σ:=σ) (K:=K) (k0:=k0)
+    have ih1 := Exp.weaken_subst_comm (t:=f1) (σ:=σ) (K:=K) (k0:=k0)
+    have ih2 := Exp.weaken_subst_comm (t:=f2) (σ:=σ) (K:=K,x) (k0:=k0)
+    simp [Exp.subst, Exp.rename, ih0, ih1]
+    exact ih2
 
 theorem Exp.weaken_subst_comm_base {t : Exp s1} {σ : Subst s1 s2} :
   (t.subst σ).rename (Rename.succ (k:=k0)) = (t.rename Rename.succ).subst (σ.lift (k:=k0)) :=
@@ -177,14 +205,6 @@ theorem Subst.comp_lift {σ1 : Subst s1 s2} {σ2 : Subst s2 s3} {k : Kind} :
         lhs; simp only [Subst.comp, Subst.lift_there_var_eq]
       simp only [Subst.lift_there_var_eq]
       simp only [Exp.weaken_subst_comm_base, Subst.comp]
-  · intro x
-    cases x with
-    | here => rfl
-    | there x0 =>
-      conv =>
-        lhs; simp only [Subst.comp, Subst.lift_there_tvar_eq]
-      simp only [Subst.lift_there_tvar_eq]
-      simp only [Ty.weaken_subst_comm_base, Subst.comp]
 
 theorem Subst.comp_liftMany {σ1 : Subst s1 s2} {σ2 : Subst s2 s3} {K : Sig} :
   (σ1.liftMany K).comp (σ2.liftMany K) = (σ1.comp σ2).liftMany K := by
@@ -197,12 +217,16 @@ theorem Subst.comp_liftMany {σ1 : Subst s1 s2} {σ2 : Subst s2 s3} {K : Sig} :
 theorem Ty.subst_comp {t : Ty s1} {σ1 : Subst s1 s2} {σ2 : Subst s2 s3} :
   (t.subst σ1).subst σ2 = t.subst (σ1.comp σ2) := by
   induction t generalizing s2 s3 with
-  | top => rfl
-  | tvar => simp [Ty.subst, Subst.comp]
+  | base => rfl
   | arrow _ _ ih0 ih1 =>
     simp_all [Ty.subst]
-  | forall_ _ _ ih0 ih1 =>
-    simp_all [Ty.subst, Subst.comp_lift]
+  | prod _ _ ih0 ih1 =>
+    simp_all [Ty.subst]
+  | sum _ _ ih0 ih1 =>
+    simp_all [Ty.subst]
+  | list _ ih0 =>
+    simp_all [Ty.subst]
+  | unit => rfl
 
 theorem Exp.subst_comp {t : Exp s1} {σ1 : Subst s1 s2} {σ2 : Subst s2 s3} :
   (t.subst σ1).subst σ2 = t.subst (σ1.comp σ2) := by
@@ -212,28 +236,55 @@ theorem Exp.subst_comp {t : Exp s1} {σ1 : Subst s1 s2} {σ2 : Subst s2 s3} :
     simp_all [Exp.subst, Ty.subst_comp, Subst.comp_lift]
   | app _ _ ih0 ih1 =>
     simp_all [Exp.subst]
-  | tabs _ _ ih0 =>
+  | let_ _ _ ih0 ih1 =>
+    simp_all [Exp.subst, Subst.comp_lift]
+  | letrec _ _ _ ih0 ih1 =>
     simp_all [Exp.subst, Ty.subst_comp, Subst.comp_lift]
-  | tapp _ _ ih0 =>
-    simp_all [Exp.subst, Ty.subst_comp]
+  | pair _ _ ih0 ih1 =>
+    simp_all [Exp.subst]
+  | fst _ ih0 =>
+    simp_all [Exp.subst]
+  | snd _ ih0 =>
+    simp_all [Exp.subst]
+  | inl _ ih0 =>
+    simp_all [Exp.subst]
+  | inr _ ih0 =>
+    simp_all [Exp.subst]
+  | case_ _ _ _ ih0 ih1 ih2 =>
+    simp_all [Exp.subst, Subst.comp_lift]
+  | nil => rfl
+  | cons _ _ ih0 ih1 =>
+    simp_all [Exp.subst]
+  | foldr _ _ _ ih0 ih1 ih2 =>
+    simp_all [Exp.subst]
+  | unit => rfl
+  | fix _ ih0 =>
+    simp_all [Exp.subst, Subst.comp_lift]
+  | num => rfl
+  | succ _ ih0 =>
+    simp_all [Exp.subst]
+  | ifz _ _ _ ih0 ih1 ih2 =>
+    simp_all [Exp.subst, Subst.comp_lift]
 
 theorem Subst.lift_id :
   (Subst.id (s:=s)).lift (k:=k) = Subst.id := by
   apply Subst.funext
   · intro x
     cases x <;> rfl
-  · intro x
-    cases x <;> rfl
 
 theorem Ty.subst_id {t : Ty s} :
   t.subst Subst.id = t := by
   induction t with
-  | top => rfl
-  | tvar => simp [Ty.subst, Subst.id]
+  | base => rfl
   | arrow _ _ ih0 ih1 =>
     simp_all [Ty.subst]
-  | forall_ _ _ ih0 ih1 =>
-    simp_all [Ty.subst, Subst.lift_id]
+  | prod _ _ ih0 ih1 =>
+    simp_all [Ty.subst]
+  | sum _ _ ih0 ih1 =>
+    simp_all [Ty.subst]
+  | list _ ih0 =>
+    simp_all [Ty.subst]
+  | unit => rfl
 
 theorem Exp.subst_id {t : Exp s} :
   t.subst Subst.id = t := by
@@ -243,9 +294,34 @@ theorem Exp.subst_id {t : Exp s} :
     simp_all [Exp.subst, Ty.subst_id, Subst.lift_id]
   | app _ _ ih0 ih1 =>
     simp_all [Exp.subst]
-  | tabs _ _ ih0 =>
+  | let_ _ _ ih0 ih1 =>
+    simp_all [Exp.subst, Subst.lift_id]
+  | letrec _ _ _ ih0 ih1 =>
     simp_all [Exp.subst, Ty.subst_id, Subst.lift_id]
-  | tapp _ _ ih0 =>
-    simp_all [Exp.subst, Ty.subst_id]
+  | pair _ _ ih0 ih1 =>
+    simp_all [Exp.subst]
+  | fst _ ih0 =>
+    simp_all [Exp.subst]
+  | snd _ ih0 =>
+    simp_all [Exp.subst]
+  | inl _ ih0 =>
+    simp_all [Exp.subst]
+  | inr _ ih0 =>
+    simp_all [Exp.subst]
+  | case_ _ _ _ ih0 ih1 ih2 =>
+    simp_all [Exp.subst, Subst.lift_id]
+  | nil => rfl
+  | cons _ _ ih0 ih1 =>
+    simp_all [Exp.subst]
+  | foldr _ _ _ ih0 ih1 ih2 =>
+    simp_all [Exp.subst]
+  | unit => rfl
+  | fix _ ih0 =>
+    simp_all [Exp.subst, Subst.lift_id]
+  | num => rfl
+  | succ _ ih0 =>
+    simp_all [Exp.subst]
+  | ifz _ _ _ ih0 ih1 ih2 =>
+    simp_all [Exp.subst, Subst.lift_id]
 
-end Fsub
+end MiniML
